Re-add the computational model without promise-free optimization

ArchSemArm/tests/UMPromisingTest.v
@@ -153,6 +153,14 @@ Module LDR. (* LDR X0, [X1, X0] at 0x500, loading from 0x1000 *)
     vm_compute (_ <$> _).
     reflexivity.
   Qed.
+
+  Definition test_results_pf :=
+    UMPromising_cert_c_pf arm_sem fuel n_threads termCond initState.
+
+  Goal reg_extract R0 0%fin <$> test_results_pf = Listset [Ok 0x2a%Z].
+    vm_compute (_ <$> _).
+    reflexivity.
+  Qed.
 End LDR.
 
 Module STRLDR. (* STR X2, [X1, X0]; LDR X0, [X1, X0] at 0x500, using address 0x1100 *)
@@ -187,6 +195,14 @@ Module STRLDR. (* STR X2, [X1, X0]; LDR X0, [X1, X0] at 0x500, using address 0x1
     UMPromising_cert_c arm_sem fuel n_threads termCond initState.
 
   Goal reg_extract R0 0%fin <$> test_results ≡ Listset [Ok 0x2a%Z].
+    vm_compute (_ <$> _).
+    set_solver.
+  Qed.
+
+  Definition test_results_pf :=
+    UMPromising_cert_c_pf arm_sem fuel n_threads termCond initState.
+
+  Goal reg_extract R0 0%fin <$> test_results_pf ≡ Listset [Ok 0x2a%Z].
     vm_compute (_ <$> _).
     set_solver.
   Qed.
@@ -261,6 +277,16 @@ Module MP.
     vm_compute (elements _).
     apply NoDup_Permutation; try solve_NoDup; set_solver.
   Qed.
+
+  Definition test_results_pf :=
+    UMPromising_cert_c_pf arm_sem fuel n_threads termCond initState.
+
+  Goal elements (regs_extract [(1%fin, R5); (1%fin, R2)] <$> test_results) ≡ₚ
+    [Ok [0x0%Z;0x2a%Z]; Ok [0x0%Z;0x0%Z]; Ok [0x1%Z; 0x2a%Z]; Ok [0x1%Z; 0x0%Z]].
+  Proof.
+    vm_compute (elements _).
+    apply NoDup_Permutation; try solve_NoDup; set_solver.
+  Qed.
 End MP.
 
 Module MPDMBS.
@@ -327,6 +353,17 @@ Module MPDMBS.
 
   Definition test_results :=
     UMPromising_cert_c arm_sem fuel n_threads termCond initState.
+
+  (** The test is fenced enough, the 0x1;0x0 outcome is impossible*)
+  Goal elements (regs_extract [(1%fin, R5); (1%fin, R2)] <$> test_results) ≡ₚ
+    [Ok [0x0%Z;0x2a%Z]; Ok [0x0%Z;0x0%Z]; Ok [0x1%Z; 0x2a%Z]].
+  Proof.
+    vm_compute (elements _).
+    apply NoDup_Permutation; try solve_NoDup; set_solver.
+  Qed.
+
+  Definition test_results_pf :=
+    UMPromising_cert_c_pf arm_sem fuel n_threads termCond initState.
 
   (** The test is fenced enough, the 0x1;0x0 outcome is impossible*)
   Goal elements (regs_extract [(1%fin, R5); (1%fin, R2)] <$> test_results) ≡ₚ
